...

interface_abstraction/Spoofing.thy
@@ -1,34 +1,34 @@
 theory Spoofing
-imports Network
+imports Network_View
 begin
 
 section{*Can hosts spoof?*}
-  definition host_cannot_spoof :: "'v network \<Rightarrow> 'v interface \<Rightarrow> bool" where
-    "host_cannot_spoof N start \<equiv> \<forall> spoofed dst. spoofed \<noteq> entity start \<longrightarrow> reachable N (spoofed, dst) start \<subseteq> networkboxes (succ N start)"
+  definition host_cannot_spoof_ingress :: "'v network \<Rightarrow> 'v interface \<Rightarrow> bool" where
+    "host_cannot_spoof_ingress N start \<equiv> \<forall> spoofed dst. spoofed \<noteq> entity start \<longrightarrow> reachable N (spoofed, dst) start \<subseteq> networkboxes (succ N start)"
 
 
   (*if spoofed adresses exist ...*)
-  lemma "\<exists> spoofed. spoofed \<noteq> entity start \<Longrightarrow> host_cannot_spoof N start \<Longrightarrow> succ N start = networkboxes (succ N start)"
+  lemma "\<exists> spoofed. spoofed \<noteq> entity start \<Longrightarrow> host_cannot_spoof_ingress N start \<Longrightarrow> succ N start = networkboxes (succ N start)"
     apply(rule succ_subset_networkboxes)
-    apply(simp add: host_cannot_spoof_def)
+    apply(simp add: host_cannot_spoof_ingress_def)
     apply(erule exE)
     using succ_subseteq_reachable by fast
 
   (*if the adress space is so small that there is only one adress, a host cannot spoof (obviously)*)
-  lemma "\<not> (\<exists> spoofed. spoofed \<noteq> entity start) \<Longrightarrow> host_cannot_spoof N start"
-    by(simp add: host_cannot_spoof_def)
+  lemma "\<not> (\<exists> spoofed. spoofed \<noteq> entity start) \<Longrightarrow> host_cannot_spoof_ingress N start"
+    by(simp add: host_cannot_spoof_ingress_def)
     
 
   text{*if all networkboxes connected to start block spoofing, start cannot spoof*}
   lemma 
     assumes connected_to_networkboxes: "succ N start = networkboxes (succ N start)" 
       and   no_fwd_spoofed: "\<forall> spoofed dst. spoofed \<noteq> entity start \<longrightarrow> (\<forall> first_hop \<in> succ N start. (forward N (spoofed, dst) first_hop) = {})"
-    shows "host_cannot_spoof N start"
+    shows "host_cannot_spoof_ingress N start"
     proof -
       {
       have "\<forall> spoofed dst. spoofed \<noteq> entity start \<longrightarrow> (\<forall> first_hop \<in> succ N start. (forward N (spoofed, dst) first_hop) = {}) \<Longrightarrow>
-                host_cannot_spoof N start"
-      apply(simp add: host_cannot_spoof_def)
+                host_cannot_spoof_ingress N start"
+      apply(simp add: host_cannot_spoof_ingress_def)
       apply(clarify)
       apply(erule reachable_induct)
       apply(simp)
@@ -40,17 +40,51 @@ section{*Can hosts spoof?*}
       from this no_fwd_spoofed show ?thesis by simp
     qed
 
+ lemma assumes wf_N: "wellformed_network N"
+  shows "host_cannot_spoof_ingress N start \<longleftrightarrow> (\<forall> spoofed dst. spoofed \<noteq> entity start \<longrightarrow> (\<forall>first_hop\<in>succ N start. traverse N (spoofed, dst) first_hop \<subseteq> succ N start))"
+  (is "?L \<longleftrightarrow> ?R")
+  proof
+    assume nospoof: "?L"
+    { fix spoofed dst
+      assume spoofed: "spoofed \<noteq> entity start"
+      from nospoof spoofed have "\<forall>dst. reachable N (spoofed, dst) start \<subseteq> networkboxes (succ N start)"
+        by(simp add: host_cannot_spoof_ingress_def)
+      hence "\<forall>dst. reachable N (spoofed, dst) start \<subseteq> succ N start" using subset_trans networkboxes_subset by metis
+      from this reachable_subset_start_iff[OF wf_N] have "\<And>dst. \<forall>first_hop\<in>succ N start. traverse N (spoofed, dst) first_hop \<subseteq> succ N start" by simp
+    }
+    thus "?R" by simp
+    next
+    assume notraverese: "?R"
+    { fix spoofed dst
+      assume spoofed: "spoofed \<noteq> entity start"
+      from notraverese spoofed have "\<forall>first_hop\<in>succ N start. traverse N (spoofed, dst) first_hop \<subseteq> succ N start"
+        by(simp add: host_cannot_spoof_ingress_def)
+      from this reachable_subset_start_iff[OF wf_N, symmetric] have "reachable N (spoofed, dst) start \<subseteq> succ N start" by simp
+    }
+    (*networkboxes*)
+    thus "?L"
+      apply(simp add: host_cannot_spoof_ingress_def) 
+oops
 
-(*
   lemma assumes wf_N: "wellformed_network N"
-    shows "host_cannot_spoof N start \<Longrightarrow> \<forall> spoofed dst. spoofed \<noteq> entity start \<longrightarrow> (\<forall> first_hop \<in> succ N start. (forward N (spoofed, dst) first_hop) = {})"
-    apply(simp add: host_cannot_spoof_def reachable_eq_rtrancl_view2[OF wf_N] view_def)
+    and nospoof: "host_cannot_spoof_ingress N start"
+    and spoofed: "spoofed \<noteq> entity start"
+    shows "\<forall> first_hop \<in> succ N start. (forward N (spoofed, dst) first_hop) = {}"
+    proof -
+      from nospoof spoofed have "\<forall>dst. reachable N (spoofed, dst) start \<subseteq> networkboxes (succ N start)"
+        by(simp add: host_cannot_spoof_ingress_def)
+      hence "\<forall>dst. reachable N (spoofed, dst) start \<subseteq> succ N start" using subset_trans networkboxes_subset by metis
+      from this reachable_subset_start_iff[OF wf_N] have "\<And>dst. \<forall>first_hop\<in>succ N start. traverse N (spoofed, dst) first_hop \<subseteq> succ N start" by simp
+      from this traverse_def have "\<And>dst p first_hop. first_hop\<in>succ N start \<Longrightarrow> p\<in>forward N (spoofed, dst) first_hop \<Longrightarrow> 
+        succ N \<lparr>entity = entity first_hop, port = p\<rparr> \<subseteq> succ N start" by blast
+
+    show ?thesis
     apply(clarsimp)
     apply(erule allE)
     apply(auto)
     (*does not hold?  reachable start \<subseteq> succ start \<Longrightarrow> no forwarding to connected ports*)
     oops
-*)
+
 
 
 end
